checker/builtins.mli
@@ -1,2 +1,4 @@
 (* Registering built-in checkers. *)
 val register : unit -> unit
+
+val tauto : MTypes.bounds -> MTypes.clause -> bool
