checker/corresp.ml
@@ -1,0 +1,95 @@
+(* Check correspondence between a model (with inferences)
+ * and the initial clauses of a resolution proof. *)
+module GL = Genlex
+module MT = MTypes
+module M = Model
+module H = Hashtbl
+module A = DynArray
+
+let lmap_of_model model =
+  let lmap = H.create 3037 in
+  H.add lmap 254 (MT.Pos MT.CTrue) ;
+  M.lits_iteri (fun i _ lit -> H.add lmap (255+i) lit) model ;
+  lmap
+
+let clause_table clauses =
+  let ctable = H.create 11437 in
+  H.add ctable [MT.Pos MT.CTrue] () ;
+  List.iter (fun cl -> H.add ctable cl ()) clauses ;
+  ctable
+  
+let get_lit lmap k =
+  try
+    H.find lmap k 
+  with Not_found ->
+    failwith
+      (Format.sprintf "Unidentified literal identifier %d." k)
+
+let tlit lmap = parser
+  | [< 'GL.Kwd "-" ; 'GL.Int k >] ->
+      MT.negate (get_lit lmap k)
+  | [< 'GL.Int k >] -> (get_lit lmap k)
+
+
+let tclause lmap tokens =
+  let rec aux = parser
+    | [< 'GL.Int 0 >] -> []
+    | [< l = (tlit lmap) ; ls = aux >] -> l :: ls
+    | [< >] -> [] in
+  aux tokens
+
+let rec tantecedents tokens = 
+  let rec aux = parser
+  | [< 'GL.Int 0 >] -> []
+  | [< 'GL.Int k ; ks = aux >] -> k :: ks in
+  aux tokens
+
+let tentry lmap = parser
+  | [< 'GL.Int id ; cl = tclause lmap ; ants = tantecedents >] ->
+      (id, cl, ants)
+
+let check_clause model cltable clause =
+  begin
+    if !COption.verbosity > 1
+    then
+      let fmt = Format.std_formatter in
+      Format.fprintf fmt "Checking %s@."
+        (M.string_of_clause model clause)
+  end ;
+  try
+    let _ = H.find cltable clause in
+    true
+  with Not_found ->
+    if Builtins.tauto (M.get_bounds model) clause then
+      true
+    else
+      begin
+        if !COption.verbosity > 0
+        then
+          let fmt = Format.err_formatter in
+          Format.fprintf fmt "Failure - unjustified clause: %s@."
+            (M.string_of_clause model clause)
+        else
+          () ;
+        false
+      end
+
+let check_entry model cltable (_, cl, ants) =
+  match ants with
+  | [] -> check_clause model cltable cl
+  | _ -> true
+
+let check model clauses tokens =
+  let lmap = lmap_of_model model
+  and ctable = clause_table clauses in
+  let rec check_aux tokens =
+    match Stream.peek tokens with
+    | None ->
+      (* Checked all entries in the resolution proof. *)
+      true
+    | _ ->
+      (* Get the next entry. *)
+      let entry = tentry lmap tokens in
+      check_entry model ctable entry && check_aux tokens
+  in
+  check_aux tokens
