checker/corresp.mli
@@ -1,0 +1,4 @@
+(* Check correspondence between a model (with inferences)
+ * and the initial clauses of a resolution proof. *)
+val check : Model.t -> MTypes.clause list -> 
+  Genlex.token Stream.t -> bool
